w64 instance

proof/examples/zk/abstract/Instance_W64.ec
@@ -7,7 +7,8 @@ require import BitEncoding.
 import BS2Int.
 
 op P : int.
-axiom P_small : 0 <= P < W64.max_uint.
+axiom P_small1 : 0 <= P.
+axiom P_small2 : P < W64.modulus.
 axiom P_prime : prime P.
 
 require import Fp_small.
@@ -19,17 +20,18 @@ clone import Abstract_exp_proof_8 as ExpW64 with type R  <- W64.t,
                                                  op bitsR <- W64.bits2w,
                                                  op P <- P
 proof*.
-
 realize Rsize_max. smt(). qed.
 realize Rsize_pos. smt(). qed.
 realize valr_pos. smt (@W64). qed.
 realize iii.  smt (@W64). qed.
-realize valr_ofint.  
-progress. 
+realize valr_ofint.  progress.
 progress. rewrite /valR. rewrite /of_int. 
 have ->: (w2bits ((bits2w (int2bs 64 x)))%W64) 
- = (int2bs 64 x). smt.
-admit.
+ = (int2bs 64 x). smt. 
+rewrite int2bsK. auto. 
+progress. 
+have : P < W64.modulus. apply P_small2.
+simplify. smt(). auto.
 qed.
 realize P_prime. apply P_prime. qed.
 realize ofint_valr. progress. smt. qed.
@@ -43,11 +45,106 @@ realize Zp.Sub.valP. admitted.
 realize Zp.Sub.valK. admitted.
 realize Zp.Sub.insubW. admitted.
 
-require import Fp_small_proof.
+import Zp.
+(* require import Fp_small_proof. *)
+op as_word (x : bool) : W64.t  = x ? W64.one : W64.zero.
+op ith_bitword64 (n : W64.t) (x : int)  : W64.t = as_word (n.[x]).
+op (^) (x : zp)(n : W64.t) : zp = inzp (asint x ^ W64.to_uint n).
+print t.
+
+module ASpecFp = {
+
+  proc ith_bit (k:W64.t, ctr:int) : W64.t = {
+    return ith_bitword64 k ctr;
+  }
+
+  proc swapw (x1:W64.t, x2:W64.t, toswap:bool) : W64.t * W64.t = {
+    return toswap ? (x2,x1) : (x1,x2);
+  }
+  
+  proc mulm(a b: zp): zp = {
+    var r;
+    r <- a * b;
+    return r;
+  }
+}.
 
 
 
-print W64.
+
+(* minu_one  twos_compl to_uint_and_mod*)
+lemma qqq x : 0 < x < 64 => W64.one.[x] = false.
+progress. timeout 20. smt.
+qed.
+
+lemma exp_ithbit :
+ equiv[ M.ith_bit ~ ASpecFp.ith_bit    : arg{2}.`1 = arg{1}.`1 /\  arg{2}.`2 = W64.to_uint arg{1}.`2 
+    /\ 0 <= ctr{2} < 64 ==> ={res} /\ (res{2} = W64.one \/ res{2} = W64.zero) ].
+    symmetry.
+proc. 
+wp. skip. 
+progress.
+rewrite /ith_bitword64.
+rewrite /as_word.
+rewrite /truncateu8.
+have -> : (to_uint (ctr{2} `&` (of_int 63)%W64))
+  = (to_uint ctr{2} %% 2 ^ 6).
+rewrite - to_uint_and_mod. auto.
+smt. simplify.
+have -> : (of_int (to_uint ctr{2} %% 64))%W8 = (of_int (to_uint ctr{2}))%W8.
+smt.
+rewrite /(`>>`).
+rewrite /(`>>>`).
+rewrite /W64.(`&`).
+rewrite /map2.
+case (k{2}.[to_uint ctr{2}]).
+progress.
+apply W64.ext_eq.
+progress.
+rewrite initiE. auto.
+simplify.
+rewrite initiE. auto.
+simplify.
+case (x = 0).
+progress. smt. 
+progress.
+have -> : W64.one.[x] = false. 
+smt (qqq).
+auto.
+progress.
+apply W64.ext_eq.
+progress.
+rewrite initiE. auto.
+simplify.
+rewrite initiE. auto.
+simplify.
+case (x = 0).
+progress. smt. 
+progress. 
+smt (qqq).
+smt().
+qed.    
+
+abbrev ImplWord2 (x : W64.t) (y : int) = W64.to_uint x = y.
+abbrev ImplFp2 (a : W64.t) (b : zp) = ImplWord2 a (asint b).
+
+import W64.
+
+equiv mulm_spec:
+ M.mulm ~ ASpecFp.mulm:
+  ImplWord2 p{1} P /\ ImplFp2 a{1} a{2} /\ ImplFp2 b{1} b{2} ==> ImplFp2 res{1} res{2}.
+proof.
+proc; simplify; wp; skip => &1 &2 /> Hp Ha Hb /=.
+rewrite /DIV_64 /MUL_64 /wdwordu /flags_w2 /flags_w /rflags_undefined /rflags_of_mul Hp /= of_uintK /mulu /=.
+have ->: (to_uint (mulhi a{1} b{1}) * 18446744073709551616 + to_uint (a{1} * b{1})) = to_uint a{1} * to_uint b{1}.
+ by rewrite -mulhiP /mulu /#.
+rewrite modz_small.
+ by move: to_uint_cmp modz_cmp; smt.
+by rewrite mulE Ha Hb.
+qed.
+
+
+
 lemma pre_fin_real : 
  equiv[ Spec.expm ~ M7(M).expm :
             valR m{2} = P /\
@@ -75,7 +172,6 @@ rewrite /as_word. simplify.
 smt (@W64).  
 rewrite /as_word. simplify.
 smt (@W64).  
-
 symmetry.
 transitivity ASpecFp.ith_bit 
   (={arg} ==> ={res})
@@ -85,19 +181,50 @@ progress. smt(). smt().
 proc. skip. progress. rewrite /ith_bitR. rewrite /ith_bitword64.
 rewrite /ith_bit. rewrite /as_w64. 
 rewrite /as_word.
-have -> : nth witness (w2bits k{2}) ctr{2}  = k{2}.[ctr{2}].
-
+have -> : nth false (w2bits k{2}) ctr{2}  = k{2}.[ctr{2}].
+smt.
 auto.
+symmetry.
+conseq exp_ithbit.
+progress.
+symmetry.
+transitivity ASpecFp.mulm
+  (={arg} ==> ={res})    
+  (ImplWord2 p{2}  P /\ ImplFp2 a{2} a{1} /\ ImplFp2 b{2} b{1} ==> ImplFp2 res{2} res{1}).
+progress. smt(). smt().
+proc. wp. skip. progress.
+symmetry. conseq mulm_spec. 
+progress.
+qed.
 
 
 
-
-
-admit. 
-
-
-admit.
-
-auto.
+lemma fin_real : 
+ equiv[ Spec.expm ~ M.expm :
+            valR m{2} = P /\
+            ImplFp x{2} a{1} /\ b{1} = valR n{2} /\ valR x{2} < P ==>
+            ImplFp res{2} res{1}].
+transitivity M7(M).expm
+  (valR m{2} = P /\
+            ImplFp x{2} a{1} /\ b{1} = valR n{2} /\ valR x{2} < P ==>
+            ImplFp res{2} res{1})
+ (={arg} ==> ={res}).
+progress. smt(). smt().
+conseq pre_fin_real.
+proc. sim.
+seq  7  9 : (={x1,x2,x3,x4,d,ctr,n,m}). sim. wp.
+call (_:true). wp.  skip. progress. wp.  sp. call (_:true). wp.  skip. progress. skip.
+progress. rewrite /oneR. smt(@W64). smt(@W64). 
+while (={x1,x2,x3,x4,d,ctr,n,m}). wp.
+call (_:true). wp. skip. progress.
+call (_:true). wp. skip. progress. wp.
+call (_:true). wp. skip. progress.
+call (_:true). wp. skip. progress.
+call (_:true). wp. skip. progress.
+wp.
+call (_:true). wp. skip. progress.
+call (_:true). wp. skip. progress.
+wp. skip. progress. smt(@W64).
+skip. progress.
 qed.
 
